\section*{Section~\ref{S:cases}}
\subsection*{Progress Check \ref{pr:n-even-odd}}
\textbf{Proposition}. \emph{For each integer $n$, $n^2 - 5n + 7$ is an odd integer}.

\begin{myproof}
Let $n$ be an integer.  We will prove that $n^2 - 5n + 7$ is an odd integer by examining the case where $n$ is even and the case where $n$ is odd.

\noindent
In the case where $n$ is even, there exists an integer $m$ such that $n = 2m$.  So in this case,
\[
\begin{aligned}
n^2 - 5n + 7 &= \left( 2m \right)^2 - 5 \left( 2m \right) + 7 \\
             &= 4m^2 - 10m + 6 + 1 \\
             &= 2 \left(2m^2 - 5m + 3 \right) + 1.
\end{aligned}
\]
Since $\left( 2m^2 - 5m + 3 \right)$ is an integer, the last equation shows that if $n$ is even, then $n^2 - 5n + 7$ is odd.

In the case where $n$ is odd, there exists an integer $m$ such that $n = 2m +1$.  So in this case,
\[
\begin{aligned}
n^2 - 5n + 7 &= \left( 2m + 1 \right)^2 - 5 \left( 2m + 1 \right) + 7 \\
             &= 4m^2 - 6m + 3 \\
             &= 2 \left(2m^2 - 3m + 1 \right) + 1.
\end{aligned}
\]
Since $\left( 2m^2 - 3m + 1 \right)$ is an integer, the last equation shows that if $n$ is odd, then $n^2 - 5n + 7$ is odd.  Hence, by using these two cases, we have shown that for each integer $n$, $n^2 - 5n + 7$ is an odd integer.
\end{myproof}



%\subsection*{Progress Check \ref{pr:cases2}}
%\textbf{Proposition}.  \emph{For all real numbers $a$ and $b$, if $ab = 0$, then $a = 0$ or $b = 0$.}
%
%\begin{myproof}
%We let $a$ be a real number and assume that $ab = 0$.  We will prove that $a = 0$ or 
%$b = 0$ by considering two cases:  (1) $a = 0$, and (2) $a \ne 0$.
%
%When $a = 0$, the conclusion of the proposition is true and so there is nothing to prove.  When $a \ne 0$, we can multiply both sides of the equation $ab = 0$ by $\dfrac{1}{a}$ and obtain
%\[
%\begin{aligned}
%\frac{1}{a} \cdot ab &= \frac{1}{a} \cdot 0 \\
%                    b & = 0.
%\end{aligned}
%\]
%This proves that if $ab = 0$, then $a = 0$ or $b = 0$.
%\end{myproof}




\subsection*{Progress Check~\ref{pr:absvalue}}
\begin{enumerate}
  \item $|4.3| = 4.3$ and $|-\pi| = \pi$
  \item \begin{enumerate}
    \item $t = 12$ or $t = -12$.
    \item $t + 3 = 5$ or $t + 3 = -5$.  So $t = 2$ or $t = -8$.
    \item $t - 4 = \dfrac{1}{5}$ or $t - 4 = -\dfrac{1}{5}$.  So $t = \dfrac{21}{5}$ or 
$t = \dfrac{19}{5}$.
    \item $3t - 4 = 8$ or $3t - 4 = -8$.  So $t = 4$ or $t = -\dfrac{4}{3}$.
\end{enumerate}
\end{enumerate}
\hbreak

\endinput
