\section*{Section~\ref{S:functionsonsets}}

\subsection*{Progress Check~\ref{prog:functionsandsets}}
\begin{multicols}{2}
\begin{enumerate}
\item $f ( A ) = \left\{ s, t \right\}$
\item $f ( B ) = \left\{ f ( x ) \mid x \in B \right\} = \left\{ s \right\}$
\end{enumerate}
\end{multicols}

\begin{enumerate} \setcounter{enumi}{2}
\item $f^{-1} ( C ) = \left\{ x \in S \mid f ( x ) \in C \right\} = 
                                 \left\{ a, b, c, d \right\}$
\item $f^{-1} ( D ) = \left\{ x \in S \mid f ( x ) \in D \right\} = 
                                 \left\{ a, d \right\}$
\end{enumerate}




\subsection*{Progress Check~\ref{prog:setsandfunctions}}
\begin{enumerate}
\item \begin{multicols}{4}
$f ( 0 ) = 2$

$f ( 1 ) = 3$

$f ( 2 ) = 6$

$f ( 3 ) = 3$

$f ( 4 ) = 2$

$f ( 5 ) = 3$

$f ( 6 ) = 6$

$f ( 7 ) = 3$
\end{multicols}

\item \begin{enumerate}
\item \begin{multicols}{2}
$f ( A ) = \left\{ 2, 3, 6 \right\}$

$f ( B ) = \left\{ 2, 3, 6 \right\}$

$f^{-1} ( C ) = \left\{ 0, 1, 3, 4, 5, 7 \right\}$

$f^{-1} ( D ) = \left\{ 1, 3, 5, 7 \right\}$
\end{multicols}
\end{enumerate}

\item \begin{enumerate}
\item \begin{multicols}{2}
$f ( A  \cap  B ) = \left\{ 2 \right\}$

$f ( A ) \cap f ( B ) = \left\{ 2, 3, 6 \right\}$
\end{multicols}
So in this case, 
$f ( A \cap B ) \subseteq f ( A ) \cap f ( B )$.

\item \begin{multicols}{2}

$f ( A )  \cup f ( B ) = \left\{ 2, 3, 6 \right\}$

$f ( A \cup B ) = \left\{ 2, 3, 6 \right\}$
\end{multicols}
So in this case, $f ( A \cup B ) = f ( A ) \cup f ( B )$.

\item 
$f^{-1} ( C ) \cap f^{-1} ( D ) = 
f^{-1} ( C \cap D ) = \left\{ 1, 3, 5, 7 \right\}$.
So in this case, 
$f^{-1} ( C \cap D ) = f^{-1} ( C ) \cap f^{-1} ( D )$.

\item
$f^{-1} ( C ) \cup f^{-1} ( D ) = 
f^{-1} ( C \cup D ) = \left\{ 0, 1, 3, 4, 5, 7 \right\}$.
So in this case, 
$f^{-1} ( C \cup D ) = f^{-1} ( C ) \cup f^{-1} ( D )$.
\end{enumerate}


\item $f ( A ) = \left\{ 2, 3, 6 \right\}$.  Hence, 
$f^{-1} \!\left( f ( A ) \right) = \left\{ 0, 1, 2, 3, 4, 5, 6, 7 \right\}$.  So in this case, 
$A \subseteq f^{-1} \!\left( f ( A ) \right)$.

\item $f^{-1} ( C ) = \left\{ 0, 1, 3, 4, 5, 7 \right\}$.  So 
$f \!\left( f^{-1} ( C ) \right) = \left\{2, 3 \right\}$.  So in this case, 
$f \!\left( f^{-1} ( C ) \right) \subseteq C$.
\end{enumerate}

\hbreak


\endinput

