\section*{Section~\ref{S:moremethods}}

\subsection*{Progress Check \ref{pr:contrapositive}}
\begin{enumerate}
\item For all real numbers $a$ and $b$, if  $ab = 0$, then  $a = 0\text{  or  }b = 0$.

\item For all real numbers $a$ and $b$, if  $ab = 0$ and $a \ne 0$, $b = 0$.

\item This gives
\[
\frac{1}{a} (ab) = \frac{1}{a} \cdot 0.
\]
We now use the associative property on the left side of this equation and simplify both sides of the equation to obtain
\begin{align*}
\left( \frac{1}{a} \cdot a \right)b &= 0 \\
1 \cdot b &= 0 \\
        b &= 0
\end{align*}
Therefore, $b = 0$ and this completes the proof of a statement that is logically equivalent to the contrapositive.  Hence, we have proved the proposition.
\end{enumerate}
\hbreak



\endinput

