\documentclass[11pt]{article}
\usepackage{c://pctex/activity}

\lhead{}
\chead{\textbf{\large{Exercise 9 -- Section 6.4\\Exploring Composite Functions}}}
\rhead{}
\lfoot{\emph{Mathematical Reasoning: Writing and Proof, Third Ed.} \\Ted Sundstrom}
\cfoot{}
\rfoot{\copyright \the\year\, by Pearson Education, Inc.\\}


\begin{document}
\noindent
Let  $A$, $B$, and  $C$  be nonempty sets and let  $f\x A \to B$  and  $g\x B \to C$.

\begin{enumerate} 
\item One example is:  $A = \left\{ {a, b} \right\}$, $B = \left\{ {p, q, r} \right\}$, 
$C = \left\{ {x, y} \right\}$.

$f\x A \to B$  with  $f\left( a \right) = p$ and  $f\left( b \right) = q$.

$g\x B \to C$ with  $g\left( p \right) = x$, $g\left( q \right) = y$, and  $g\left( r \right) = x$. 

Then,
$g \circ f\x A \to C$  with  $\left( {g \circ f} \right)\left( a \right) = x$  and   
$\left( {g \circ f} \right)\left( b \right) = y$, the function  $f$  is an injection,  $g$  is not an injection, and  $g \circ f$ is an injection.

\item This is not possible.  If  $f$  is not an injection, then there exist  $s, t \in A$ with  
$s \ne t$  and  $f\left( s \right) = f\left( t \right)$.  Then,  
$g\left( {f\left( s \right)} \right) = g\left( {f\left( t \right)} \right)$ and hence, $g \circ f$
is not an injection.

\item This is not possible.  If  $g$  is not a surjection, then there exists a  $y \in C$ such that  $g\left( x \right) \ne y$ for all  $x \in B$.  So, for each  $a \in A$,  
$f\left( a \right) \in B$ and hence  $g\left( {f\left( a \right)} \right) \ne y$.  This means that  $g \circ f$ is not a surjection.

\item One example is:  $A = \left\{ {a, b} \right\}$, $B = \left\{ {p, q, r} \right\}$, 
$C = \left\{ {x, y} \right\}$.

$f\x A \to B$  with  $f\left( a \right) = p$ and  $f\left( b \right) = q$.

$g\x B \to C$ with  $g\left( p \right) = x$, $g\left( q \right) = y$, and  $g\left( r \right) = x$. 

Then, $g \circ f\x A \to C$  with  $\left( {g \circ f} \right)\left( a \right) = x$  and   
$\left( {g \circ f} \right)\left( b \right) = y$, the function  $f$  is not a surjection,  $g$  is not a surjection, and  $g \circ f$ is a surjection.

\end{enumerate}



\end{document}
