\begin{previewactivity}[\textbf{Proving that Statements Are Equivalent}] \label{PA:provingequiv} \hfill

\begin{enumerate}
\item Let $X$, $Y$, and $Z$ be statements.  Complete a truth table for  \\$\left[ {\left( {X \to Y} \right) \wedge \left( {Y \to Z} \right)} \right] \to \left( {X \to Z} \right)$.

\item Assume that  $P$, $Q$, and  $R$  are statements and that we have proven that the following conditional statements are true:
\begin{multicols}{2}
\begin{itemize}
  \item If  $P$  then  $Q$  $\left( {P \to Q} \right)$.
  \item If  $Q$  then  $R$  $\left( {Q \to R} \right)$.
  \item If  $R$  then  $P$  $\left( {R \to P} \right)$.
\end{itemize}
\end{multicols}
Explain why each of the following statements is true.
\begin{multicols}{2}
\begin{enumerate}
  \item $P$  if and only if  $Q$  $\left( {P \leftrightarrow Q} \right)$.
  \item $Q$  if and only if  $R$  $\left( {Q \leftrightarrow R} \right)$.
  \item $R$  if and only if  $P$  $\left( {R \leftrightarrow P} \right)$.
\end{enumerate}
\end{multicols} 
Remember that  $X \leftrightarrow Y$  is logically equivalent to  
$\left( {X \to Y} \right) \wedge \left( {Y \to X} \right)$.

\end{enumerate}
\end{previewactivity}
\hbreak


\endinput
